TCB/Semantics.v
@@ -6,6 +6,12 @@ Require Import LazyList.
 
 Set Implicit Arguments.
 
+(* a memory is a map from addresses to maybe byte *)
+Definition memory := N -> option byte.
+
+(* we fix the size of the header *)
+Definition header_size := 65536.
+
 (* classification of instructions *)
 
 Inductive instruction_classification (register:Type) : Type :=
@@ -25,7 +31,6 @@ Implicit Arguments Direct_jump [[register]].
 Implicit Arguments Indirect_jump [[register]].
 Implicit Arguments Invalid_instruction [[register]].
 
-Definition memory := N -> option byte.
 
 (* the state of the machine *)
 
@@ -57,198 +62,99 @@ Module Type INSTRUCTION.
   Parameter instruction: Type.
 
   (* parse an instruction *)
-  Parameter parse_instruction: byte_map -> option (instruction * nat).
+  Parameter parse_instruction: lazy_list byte -> option (instruction * nat).
+
+  Parameter instr_max_size: nat.
 
   Parameter parse_instruction_do_read:
-    forall bm instr n, parse_instruction bm = Some (instr, n) ->
-    forall n', (n' < n)%nat -> is_some (bm n').
+    forall ll instr n, parse_instruction ll = Some (instr, n) ->
+    (ll_length ll >= n)%nat.
 
   Parameter parse_instruction_only_read:
-    forall bm instr n, parse_instruction bm = Some (instr, n) ->
-    forall bm', (forall n', (n' < n)%nat -> bm n' = bm' n') ->
-      parse_instruction bm' = Some (instr, n).
+    forall ll instr n, parse_instruction ll = Some (instr, n) ->
+    forall ll',
+      ll_safe_take n ll' = ll_safe_take n ll ->
+      parse_instruction ll' = Some (instr, n).
 
-  Parameter size_instr_not_0: forall bm instr n,
-    parse_instruction bm = Some (instr, n) -> n <> O.
+  Parameter size_instr_not_0: forall ll instr n,
+    parse_instruction ll = Some (instr, n) -> n <> O.
+
+  Parameter size_instr_inf_max_size: forall ll instr n,
+    parse_instruction ll = Some (instr, n) -> (n < instr_max_size)%nat.
+
 
   Parameter classify_instruction: instruction -> instruction_classification register.
 
-  Parameter instruction_semantics: N -> instruction ->
+
+  Parameter instruction_semantics: forall code_size:N, instruction ->
     state register -> instruction_target_state register -> Prop.
+
+
+  (* the first parameter is to indicate that the n first bytes of the memory
+     cannot be written *)
+
+
+  (* an instruction cannot write in the lower code segment *)
+  Parameter sem_no_overwrite: forall code_size instr st1 st2,
+    instruction_semantics code_size instr st1 (Good_state st2) ->
+    forall n', n' < header_size + code_size -> st1.(state_mem) n' = st2.(state_mem) n'.
+
+  (* the "good" instructions can get stuck but neverr lead to a "bad state" *)
+
+  Parameter sem_not_invalid_not_bad: forall instr,
+    classify_instruction instr <> Invalid_instruction ->
+    forall code_size st,
+      ~ instruction_semantics code_size instr st Bad_state.
+
+
+  Parameter sem_OK_instr_pc: forall bm instr size,
+    parse_instruction bm = Some (instr, size) ->
+    classify_instruction instr = OK_instr ->
+    forall code_size st1 st2,
+    instruction_semantics code_size instr st1 (Good_state st2) ->
+    st2.(state_pc) = st1.(state_pc) + (N_of_nat size).
+
+  Parameter sem_Mask_instr_pc: forall bm instr size,
+    parse_instruction bm = Some (instr, size) ->
+    forall reg w,
+    classify_instruction instr = Mask_instr reg w->
+    forall code_size st1 st2,
+    instruction_semantics code_size instr st1 (Good_state st2) ->
+    st2.(state_pc) = st1.(state_pc) + (N_of_nat size).
+
+  Parameter sem_Mask_instr_reg: forall bm instr size,
+    parse_instruction bm = Some (instr, size) ->
+    forall reg w,
+    classify_instruction instr = Mask_instr reg w->
+    forall code_size st1 st2,
+    instruction_semantics code_size instr st1 (Good_state st2) ->
+    st2.(state_regs) reg = word_and w (st1.(state_regs) reg).
+
+
+  Parameter sem_Direct_jump_pc: forall bm instr size,
+    parse_instruction bm = Some (instr, size) ->
+    forall w,
+    classify_instruction instr = Direct_jump w ->
+    forall code_size st1 st2,
+    instruction_semantics code_size instr st1 (Good_state st2) ->
+    st2.(state_pc) = st1.(state_pc) + (N_of_nat size) \/
+    st2.(state_pc) = N_of_word w.
+
+  Parameter sem_Indirect_jump_pc: forall bm instr size,
+    parse_instruction bm = Some (instr, size) ->
+    forall reg,
+    classify_instruction instr = Indirect_jump reg ->
+    forall code_size st1 st2,
+    instruction_semantics code_size instr st1 (Good_state st2) ->
+    st2.(state_pc) = st1.(state_pc) + (N_of_nat size) \/
+    st2.(state_pc) = N_of_word (st1.(state_regs) reg).
+
+
 
 End INSTRUCTION.
 
 
 
-(*Fixpoint pow2 (n: nat) :=
-  match n with
-    | O => 1
-    | S n' => 2 * pow2 n'
-  end.
 
 
-Definition dividable_by_pow2 (p: nat) (n:N) :=
-  exists d:N, n = (pow2 p) * d.
-
-Lemma dividable_by_pow2_dec:
-  forall p n, {dividable_by_pow2 p n}+{~dividable_by_pow2 p n}.
-Proof.
-  unfold dividable_by_pow2.
-  intros. destruct' n as [|pos].
-  Case "0".
-  left. exists 0. zify. omega.
-  Case "Npos pos".
-  revert p.
-  induction' pos as [pos|pos|]; intros.
-  SCase "xI pos".
-  destruct' p as [|p'].
-    SSCase "0%nat".
-    left. exists (Npos pos~1). reflexivity.
-    SSCase "S p'".
-    right. intros [d H]. simpl in H. destruct (pow2 p').
-      inv H.
-      simpl in H. destruct d; inv H.
-
-   SCase "xO pos".
-   destruct' p as [|p'].
-   SSCase "0%nat".
-     left. exists (Npos pos~0). reflexivity.
-   SSCase "S p'".
-     destruct' (IHpos p') as [EXISTS|NEXISTS].
-     S3Case "left EXISTS".
-       left. destruct EXISTS as [d H].
-       exists d. simpl. destruct (pow2 p'). inv H.
-       simpl. destruct d. inv H. inv H. reflexivity.
-
-     S3Case "right NEXISTS".
-       right. intros [d H].
-       apply NEXISTS.
-       simpl in H. destruct (pow2 p'). inv H.
-       exists d. simpl. destruct d; inv H. reflexivity.
-
-  SCase "1%positive".
-   destruct' p as [|p'].
-   SSCase "0%nat".
-     left. exists 1. reflexivity.
-   SSCase "S p'".
-     right. intros [d H]. simpl in H. destruct (pow2 p'); inv H.
-     destruct d; inv H1.
-Qed.*)
-
-Definition dividable_by_32 (n:N) :=
-  exists d:N, n = 32 * d.
-
-Program Definition dividable_by_32_dec n
-  : {dividable_by_32 n} + {~dividable_by_32 n}:=
-  match n with
-    | N0 => left _
-    | Npos p~0~0~0~0~0 => left _
-    | Npos _ => right _
-  end.
-Next Obligation.
-  unfold dividable_by_32. exists 0. reflexivity.
-Qed.
-Next Obligation.
-  unfold dividable_by_32. simpl. exists (Npos p). reflexivity.
-Qed.
-Next Obligation.
-  destruct wildcard' as [wildcard'|wildcard'|]; try solve
-    [let H0 := fresh "H" in intros [[|?] H0]; simpl in H0; inv H0].
-  destruct wildcard' as [wildcard'|wildcard'|]; try solve
-    [let H0 := fresh "H" in intros [[|?] H0]; simpl in H0; inv H0].
-  destruct wildcard' as [wildcard'|wildcard'|]; try solve
-    [let H0 := fresh "H" in intros [[|?] H0]; simpl in H0; inv H0].
-  destruct wildcard' as [wildcard'|wildcard'|]; try solve
-    [let H0 := fresh "H" in intros [[|?] H0]; simpl in H0; inv H0].
-  destruct wildcard' as [wildcard'|wildcard'|]; try solve
-    [let H0 := fresh "H" in intros [[|?] H0]; simpl in H0; inv H0].
-  intro. apply (H wildcard'). reflexivity.
-Qed.
-
-
-
-(* Define the semantics of programs, parameterized by those of instruction *)
-Module Prog_Semantics (Import I: INSTRUCTION).
-
-  Inductive target_state :=
-    (* a regular state *)
-  | Normal_state: state register -> target_state
-    (* a state that should *never* be reached ! *)
-  | DANGER_STATE: target_state.
-
-
-  Definition read_instr_from_memory (mem: memory) (pc: N): option (instruction * nat) :=
-    parse_instruction (fun n => mem ((N_of_nat n) + pc)).
-
-
-
-
-
-  (* parse an instruction *)
-  Definition same_code (code_segment_size: N) (mem1 mem2: memory): Prop:=
-    forall n, n < code_segment_size -> mem1 n = mem2 n.
-
-  Definition in_code (header_size code_size: N) (st: state register) :=
-    header_size <= st.(state_pc) /\ st.(state_pc) < header_size + code_size.
-
-  Inductive step (header_size code_size: N) (st1: state register): target_state -> Prop :=
-  | Step_good: forall instr n st2,
-    in_code header_size code_size st1 ->
-    read_instr_from_memory st1.(state_mem) st1.(state_pc) = Some (instr, n) ->
-    instruction_semantics (header_size + code_size) instr st1 (Good_state st2) ->
-    (* we allow any modification of the memory outside of the code
-       segment because of multi threading *)
-    forall m2', same_code (header_size + code_size) m2' st2.(state_mem) ->
-    step header_size code_size st1
-      (Normal_state {| state_mem := m2';
-                       state_pc := st2.(state_pc);
-                       state_regs :=st2.(state_regs) |})
-    (* if no instruction can be read, something wrong is hapening *)
-  | Step_cannot_read_instr:
-    in_code header_size code_size st1 ->
-    read_instr_from_memory st1.(state_mem) st1.(state_pc) = None ->
-    step header_size  code_size st1 DANGER_STATE
-    (* if we can read an instruction, and its execution goes wrong, it is wrong *)
-  | Step_bad: forall instr n,
-    in_code header_size code_size st1 ->
-    read_instr_from_memory st1.(state_mem) st1.(state_pc) = Some (instr, n) ->
-    instruction_semantics (header_size + code_size) instr st1 Bad_state ->
-    step header_size code_size st1 DANGER_STATE
-
-    (* if we are in the header, it must be at a correct address *)
-  | Step_header_bad:
-    st1.(state_pc) < header_size -> ~dividable_by_32 st1.(state_pc) ->
-    step header_size code_size st1 DANGER_STATE
-
-    (* if the address in the header is correct, we can jump anywhere in the code *)
-  | Step_header_good: 
-    st1.(state_pc) < header_size -> dividable_by_32 st1.(state_pc) ->
-    forall m2 regs2 pc2,
-      same_code (header_size + code_size) st1.(state_mem) m2 ->
-      dividable_by_32 pc2 ->
-      step header_size code_size st1
-        (Normal_state {| state_mem := m2;
-                         state_pc := pc2;
-                         state_regs := regs2 |}).
-
-
-  Inductive accessible_state (header_size code_size: N)
-    (st1: state register): state register -> Prop :=
-  | AS0: accessible_state header_size code_size st1 st1
-  | ASS: forall st2 st3,
-    step header_size code_size st1 (Normal_state st2) ->
-    accessible_state header_size code_size st2 st3 ->
-    accessible_state header_size code_size st1 st3.
-
-  (* is DANGER_STATE accessible from a state ? *)
-  Inductive accessible_danger (header_size code_size: N) (st1: state register) : Prop :=
-  | AD_one_step:
-    step header_size code_size st1 DANGER_STATE ->
-    accessible_danger header_size code_size st1
-  | AD_more_steps: forall st2,
-    step header_size code_size st1 (Normal_state st2)  ->
-    accessible_danger header_size code_size st2 ->
-    accessible_danger header_size code_size st1.
-
-End Prog_Semantics.
 
