TCB/Memory.v
@@ -1,0 +1,175 @@
+Require Import Lib.
+Require Import BinaryProps.
+Require Import List.
+Require Import Program.
+Require Import LazyList.
+Require Import Semantics.
+Require Import DoOption.
+
+
+(* LIB*)
+Ltac omega' := zify; omega.
+
+
+
+Definition memory_compat_addr_ll addr ll (mem: memory):=
+  forall n, (n < ll_length ll)%nat -> ll_nth n ll = mem (addr + N_of_nat n).
+
+
+
+Lemma memory_compat_addr_ll_drop: forall addr ll mem n ll',
+  ll_safe_drop n ll = Some ll' ->
+  memory_compat_addr_ll addr ll mem ->
+  memory_compat_addr_ll (addr + N_of_nat n) ll' mem.
+Proof.
+  unfold memory_compat_addr_ll. intros.
+  erewrite ll_safe_drop_nth; eauto.
+  rewrite <- Nplus_assoc. rewrite <- N_of_plus. apply H0.
+  apply ll_safe_drop_size in H. omega.
+Qed.
+
+Lemma memory_compat_addr_ll_cons: forall addr b ll mem,
+  memory_compat_addr_ll addr (b:::ll) mem ->
+  memory_compat_addr_ll (addr + 1) ll mem.
+Proof.
+  unfold memory_compat_addr_ll. intros.
+  simpl in H.
+  specialize (H (S n)). simpl in H.
+  rewrite H. f_equal. omega'. omega.
+Qed.
+
+
+
+Hint Resolve memory_compat_addr_ll_drop memory_compat_addr_ll_cons.
+
+Module Mem(Import I : INSTRUCTION).
+
+
+  (* to read an instruction in memory, we build a list of maximal size
+     instr_size_max, and we parse it *)
+
+
+  Fixpoint build_list_from_memory (n:nat) (addr:N) (mem:memory) : lazy_list byte :=
+    match n with
+      | O => 〈〉
+      | S n' =>
+        match mem addr with
+          | None => 〈〉
+          | Some b => b ::: build_list_from_memory n' (addr + 1) mem
+        end
+    end.
+
+  Definition read_instr_from_memory (mem: memory) (pc: N): option (instruction * nat) :=
+    parse_instruction (build_list_from_memory instr_max_size pc mem).
+
+  Lemma memory_compat_read_instr addr ll mem:
+    memory_compat_addr_ll addr ll mem ->
+    forall instr size_instr,
+      parse_instruction ll = Some (instr, size_instr) ->
+      read_instr_from_memory mem addr = Some (instr, size_instr).
+  Proof.
+    intros COMPAT * PARSE.
+    unfold read_instr_from_memory.
+    remember instr_max_size as ims.
+    assert (size_instr < ims)%nat.
+      subst. eapply size_instr_inf_max_size; eauto.
+    clear Heqims.
+    eapply parse_instruction_only_read; eauto.
+    apply parse_instruction_do_read in PARSE.
+
+    assert (is_some (ll_safe_take size_instr ll)).
+    clear - PARSE. revert size_instr PARSE.
+    induction' ll as [| b ll']; simpl; intros.
+    Case "@ll_nil".
+      replace size_instr with O in * by omega. simpl. constructor.
+    Case "ll_cons b ll'".
+      destruct size_instr.
+      simpl. constructor.
+      assert (ll_length ll' >= size_instr)%nat by omega.
+      specialize (IHll' _ H). inv IHll'.
+      simpl. rewrite <- H1. constructor.
+
+
+    revert dependent ims. revert addr mem COMPAT instr size_instr PARSE H0.
+    induction' ll as [| b ll']; simpl; intros.
+    Case "@ll_nil".
+      replace size_instr with O in * by omega.
+      reflexivity.
+    Case "ll_cons b ll'".
+      destruct' size_instr.
+      SCase "0%nat".
+        reflexivity.
+      SCase "S".
+        destruct ims; [elimtype False; omega|].
+        assert (size_instr < ims)%nat by omega.
+        assert (ll_length ll' >= size_instr)%nat by omega.
+        simpl in *. inv H0; clean. inv_opt.
+        pose proof COMPAT.
+        unfold memory_compat_addr_ll in H3.
+        specialize (H3 O). replace (addr + N_of_nat 0) with addr in * by omega'.
+        rewrite <- H3;simpl;[|omega].
+        rewrite IHll'; eauto.
+        rewrite H0. reflexivity.
+  Qed.
+
+  Hint Resolve memory_compat_read_instr.
+
+
+
+  (* parse an instruction *)
+  Definition same_code (code_size: N) (mem1 mem2: memory): Prop:=
+    forall n, n < header_size + code_size -> mem1 n = mem2 n.
+
+  Lemma same_code_trans: forall code_segment_size st1 st2 st3,
+    same_code code_segment_size st1 st2 -> same_code code_segment_size st2 st3 ->
+    same_code code_segment_size st1 st3.
+  Proof.
+    unfold same_code; intros.
+    rewrite H; eauto.
+  Qed.
+
+  Lemma memory_compat_same_code ll mem1 mem2:
+    memory_compat_addr_ll header_size ll mem1 ->
+    same_code (N_of_nat (ll_length ll)) mem1 mem2 ->
+    memory_compat_addr_ll header_size ll mem2.
+  Proof.
+    unfold memory_compat_addr_ll, same_code.
+    intros.
+    rewrite H; auto.
+    apply H0. omega'.
+  Qed.
+
+  Hint Resolve memory_compat_same_code same_code_trans.
+
+
+  Definition in_code (code_size: N) (st: state register) :=
+    header_size <= st.(state_pc) /\ st.(state_pc) < header_size + code_size.
+
+
+  Lemma same_code_read_instr (mem1 mem2: memory) next_addr addr:
+    (forall addr : N, addr < next_addr -> mem1 addr = mem2 addr) ->
+    forall instr size_instr,
+      addr + N_of_nat size_instr <= next_addr ->
+      read_instr_from_memory mem1 addr = Some (instr, size_instr) ->
+      read_instr_from_memory mem2 addr = Some (instr, size_instr).
+  Proof.
+    unfold read_instr_from_memory. intros SAME * INF READ.
+    eapply parse_instruction_only_read; eauto.
+(*    pose proof READ.*)
+(*    apply parse_instruction_do_read in READ.*)
+    remember instr_max_size as ims. clear Heqims. clear READ.
+    revert dependent ims. revert dependent addr. clear instr.
+    induction' size_instr as [|size_instr]; intros.
+    Case "0%nat".
+      simpl. reflexivity.
+    Case "S size_instr".
+      simpl.
+      destruct ims; simpl.
+      reflexivity.
+      replace (mem2 addr) with (mem1 addr) in * by (apply SAME; omega').
+      destruct (mem1 addr); auto.
+      erewrite IHsize_instr; eauto. omega'.
+  Qed.
+  Hint Resolve same_code_read_instr.
+
+End Mem.
