TCB/SemanticsProg.v
@@ -1,0 +1,114 @@
+Require Import Lib.
+Require Import BinaryProps.
+Require Import List.
+Require Import Program.
+Require Import LazyList.
+Require Import Semantics.
+Require Import Memory.
+
+Definition dividable_by_32 (n:N) :=
+  exists d:N, n = 32 * d.
+
+Program Definition dividable_by_32_dec n
+  : {dividable_by_32 n} + {~dividable_by_32 n}:=
+  match n with
+    | N0 => left _
+    | Npos p~0~0~0~0~0 => left _
+    | Npos _ => right _
+  end.
+Next Obligation.
+  unfold dividable_by_32. exists 0. reflexivity.
+Qed.
+Next Obligation.
+  unfold dividable_by_32. simpl. exists (Npos p). reflexivity.
+Qed.
+Next Obligation.
+  destruct wildcard' as [wildcard'|wildcard'|]; try solve
+    [let H0 := fresh "H" in intros [[|?] H0]; simpl in H0; inv H0].
+  destruct wildcard' as [wildcard'|wildcard'|]; try solve
+    [let H0 := fresh "H" in intros [[|?] H0]; simpl in H0; inv H0].
+  destruct wildcard' as [wildcard'|wildcard'|]; try solve
+    [let H0 := fresh "H" in intros [[|?] H0]; simpl in H0; inv H0].
+  destruct wildcard' as [wildcard'|wildcard'|]; try solve
+    [let H0 := fresh "H" in intros [[|?] H0]; simpl in H0; inv H0].
+  destruct wildcard' as [wildcard'|wildcard'|]; try solve
+    [let H0 := fresh "H" in intros [[|?] H0]; simpl in H0; inv H0].
+  intro. apply (H wildcard'). reflexivity.
+Qed.
+
+
+
+(* Define the semantics of programs, parameterized by those of instruction *)
+Module Prog_Semantics (Import I: INSTRUCTION).
+
+  Module M := Mem(I).
+  Export M.
+
+  Inductive target_state :=
+    (* a regular state *)
+  | Normal_state: state register -> target_state
+    (* a state that should *never* be reached ! *)
+  | DANGER_STATE: target_state.
+
+
+  Inductive step (code_size: N) (st1: state register): target_state -> Prop :=
+  | Step_good: forall instr n st2,
+    in_code code_size st1 ->
+    read_instr_from_memory st1.(state_mem) st1.(state_pc) = Some (instr, n) ->
+    instruction_semantics (header_size + code_size) instr st1 (Good_state st2) ->
+    (* we allow any modification of the memory outside of the code
+       segment because of multi threading *)
+    forall m2', same_code code_size m2' st2.(state_mem) ->
+    step code_size st1
+      (Normal_state {| state_mem := m2';
+                       state_pc := st2.(state_pc);
+                       state_regs :=st2.(state_regs) |})
+    (* if no instruction can be read, something wrong is hapening *)
+  | Step_cannot_read_instr:
+    in_code code_size st1 ->
+    read_instr_from_memory st1.(state_mem) st1.(state_pc) = None ->
+    step code_size st1 DANGER_STATE
+    (* if we can read an instruction, and its execution goes wrong, it is wrong *)
+  | Step_bad: forall instr n,
+    in_code code_size st1 ->
+    read_instr_from_memory st1.(state_mem) st1.(state_pc) = Some (instr, n) ->
+    instruction_semantics code_size instr st1 Bad_state ->
+    step code_size st1 DANGER_STATE
+
+    (* if we are in the header, it must be at a correct address *)
+  | Step_header_bad:
+    st1.(state_pc) < header_size -> ~dividable_by_32 st1.(state_pc) ->
+    step code_size st1 DANGER_STATE
+
+    (* if the address in the header is correct, we can jump anywhere in the code *)
+  | Step_header_good:
+    st1.(state_pc) < header_size -> dividable_by_32 st1.(state_pc) ->
+    forall m2 regs2 pc2,
+      same_code code_size st1.(state_mem) m2 ->
+      dividable_by_32 pc2 ->
+      step code_size st1
+        (Normal_state {| state_mem := m2;
+                         state_pc := pc2;
+                         state_regs := regs2 |}).
+
+
+  Inductive accessible_state (code_size: N)
+    (st1: state register): state register -> Prop :=
+  | AS0: accessible_state code_size st1 st1
+  | ASS: forall st2 st3,
+    step code_size st1 (Normal_state st2) ->
+    accessible_state code_size st2 st3 ->
+    accessible_state code_size st1 st3.
+
+  (* is DANGER_STATE accessible from a state ? *)
+  Inductive accessible_danger (code_size: N) (st1: state register) : Prop :=
+  | AD_one_step:
+    step code_size st1 DANGER_STATE ->
+    accessible_danger code_size st1
+  | AD_more_steps: forall st2,
+    step code_size st1 (Normal_state st2)  ->
+    accessible_danger code_size st2 ->
+    accessible_danger code_size st1.
+
+End Prog_Semantics.
+
